# Factorization of the Quadratic Polynomial

## Given Expression
\[
4x^2 - 4x - 48
\]

---

## Step 1: Take out the common factor

All the terms have a common factor of *4*.

\[
4x^2 - 4x - 48 = 4(x^2 - x - 12)
\]

---

## Step 2: Identify values of a and b

To factor the quadratic inside the bracket:
\[
x^2 - x - 12
\]

We need two numbers *a* and *b* such that:

- \(a + b = -1\)  (coefficient of \(x\))
- \(a \cdot b = -12\) (constant term)

---

## Step 3: Find suitable values

Checking factor pairs of −12:

- \(1, -12\) → sum = −11 ❌  
- \(2, -6\) → sum = −4 ❌  
- *\(3, -4\)* → sum = −1 ✅

So,
\[
a = 3,\quad b = -4
\]

---

## Step 4: Write the factors

\[
x^2 - x - 12 = (x + 3)(x - 4)
\]

---

## Final Answer (Fully Factorized Form)

\[
\boxed{4(x + 3)(x - 4)}
\]
