### Question

Given the function:

\[
h(x) = (-4x - 3)(x - 3)
\]

Use the **Zero Product Property** to find the zeros of the function.

---

### Solution

According to the **Zero Product Property**, if the product of two factors is zero, then at least one of the factors must be zero.

\[
(-4x - 3)(x - 3) = 0
\]

Set each factor equal to zero.

#### Step 1:
\[
-4x - 3 = 0
\]

\[
-4x = 3
\]

\[
x = -\frac{3}{4}
\]

#### Step 2:
\[
x - 3 = 0
\]

\[
x = 3
\]

---

### Final Answer

The zeros of the function are:

\[
\boxed{x = -\frac{3}{4} \text{ and } x = 3}
\]
